Finish abstract support for local + ghost state

Semantics.thy
@@ -59,7 +59,8 @@ inductive silent :: "('a,'b) com \<Rightarrow> ('a,'b) com \<Rightarrow> bool"
   par1[intro]:  "c\<^sub>1 \<leadsto> c\<^sub>1' \<Longrightarrow> c\<^sub>1 || c\<^sub>2 \<leadsto> c\<^sub>1' || c\<^sub>2" |
   par2[intro]:  "c\<^sub>2 \<leadsto> c\<^sub>2' \<Longrightarrow> c\<^sub>1 || c\<^sub>2 \<leadsto> c\<^sub>1 || c\<^sub>2'" |
   parE1[intro]: "Nil || c \<leadsto> c" |
-  parE2[intro]: "c || Nil \<leadsto> c"
+  parE2[intro]: "c || Nil \<leadsto> c" |
+  thrE[intro]:  "Thread l op Nil \<leadsto> Nil" 
 inductive_cases silentE[elim]: "c\<^sub>1 \<leadsto> c\<^sub>1'"
 
 text \<open>An execution step implies the program has changed\<close>
