State.thy
@@ -90,6 +90,10 @@ text \<open>Collect all transitions where their combinations with arbitrary loca
 definition thr\<^sub>G :: "'b merge \<Rightarrow> 'b rpred \<Rightarrow> 'b rpred"
   where "thr\<^sub>G op G \<equiv> {(m,m') |m m' l l'. (op m l,op m' l') \<in> G}"
 
+text \<open>Collect all states where all local states satisfy P\<close>
+definition thr\<^sub>A :: "'b merge \<Rightarrow> 'b pred \<Rightarrow> 'b pred"
+  where "thr\<^sub>A op P \<equiv> {m. \<forall>l. op m l \<in> P}"
+
 text \<open>Lift a local transition to a global transition given the pre and post local state\<close>
 definition thr2glb :: "'b merge \<Rightarrow> 'b \<Rightarrow> 'b \<Rightarrow> 'b rpred \<Rightarrow> 'b rpred"
   where "thr2glb op l l' r \<equiv> {(m,m'). (op m l,op m' l') \<in> r}"
@@ -115,71 +119,9 @@ lemma thr_guar:
 section \<open>Auxiliary State\<close>
 
 text \<open>
-To support auxiliary state, we require an operation capable of merging two states, such
-that the real component from the first is merged with the auxiliary component of the second.
+To support auxiliary state, we require a state relation the relates two states given their
+real components are equivalent.
 \<close>
-
-
-(*
-section \<open>State Expansion\<close>
-
-definition expand\<^sub>P
-  where "expand\<^sub>P m P \<equiv> \<Union> (m ` P)"
-
-definition expand\<^sub>G
-  where "expand\<^sub>G m r G \<equiv> {(c,c'). \<exists>(b,b')\<in> G. c \<in> m b \<and> c' \<in> m b' \<and> r c c'}"
-
-definition expand\<^sub>R
-  where "expand\<^sub>R m R \<equiv> {(c,c'). \<exists>(b,b')\<in> R. c \<in> m b \<and> c' \<in> m b'}"
-
-definition valid_expand
-  where "valid_expand m r \<equiv> 
-          (\<forall>b b' c. c \<in> m b' \<longrightarrow> c \<in> m b \<longrightarrow> b = b') \<and> 
-          (\<forall>a b c. r a b \<longrightarrow> a \<in> m c \<longrightarrow> b \<in> m c \<longrightarrow> a = b)"
-
-lemma expand_stable:
-  assumes "stable R P" "valid_expand m r"
-  shows "stable (expand\<^sub>R m R) (expand\<^sub>P m P)"
-  using assms unfolding stable_def valid_expand_def expand\<^sub>P_def expand\<^sub>R_def
-  by fastforce
-
-lemma expand_wp\<^sub>\<alpha>:
-  assumes "P \<subseteq> wp\<^sub>\<alpha> \<alpha> Q" "valid_expand m r"
-  assumes \<alpha>: "vc \<alpha>' = expand\<^sub>P m (vc \<alpha>)" "beh \<alpha>' = expand\<^sub>G m r (beh \<alpha>)"
-  shows "expand\<^sub>P m P \<subseteq> wp\<^sub>\<alpha> \<alpha>' (expand\<^sub>P m Q)"
-  using assms(1,2) unfolding wp_def valid_expand_def expand\<^sub>P_def expand\<^sub>G_def \<alpha>
-  by fastforce
-
-lemma expand_guar:
-  assumes "guar\<^sub>\<alpha> \<alpha> G" "valid_expand m r"
-  assumes \<alpha>: "vc \<alpha>' = expand\<^sub>P m (vc \<alpha>)" "beh \<alpha>' = expand\<^sub>G m r (beh \<alpha>)"
-  shows "guar\<^sub>\<alpha> \<alpha>' (expand\<^sub>G m r G)"
-  using assms(1,2,3) unfolding valid_expand_def expand\<^sub>G_def \<alpha> expand\<^sub>P_def guar_def
-  by blast
-
-text \<open>Expand the state of an atomic judgement\<close>
-lemma atomic_expandI [intro]:
-  assumes "R,G \<turnstile>\<^sub>A P {\<alpha> :: ('b,'a) basic} Q"
-  assumes "valid_expand m r"
-  assumes \<alpha>: "vc \<alpha>' = expand\<^sub>P m (vc \<alpha>)" "beh \<alpha>' = expand\<^sub>G m r (beh \<alpha>)" 
-  shows "expand\<^sub>R m R,expand\<^sub>G m r G \<turnstile>\<^sub>A expand\<^sub>P m P {\<alpha>' :: ('b,'c) basic} expand\<^sub>P m Q"
-  unfolding atomic_rule_def
-proof (safe)
-  show "stable (expand\<^sub>R m R) (expand\<^sub>P m P)" 
-    using assms(1,2) expand_stable unfolding atomic_rule_def by blast
-next
-  show "stable (expand\<^sub>R m R) (expand\<^sub>P m Q)" 
-    using assms(1,2) expand_stable unfolding atomic_rule_def by blast
-next
-  fix x assume "x \<in> expand\<^sub>P m P"
-  thus "x \<in> wp\<^sub>\<alpha> \<alpha>' (expand\<^sub>P m Q)"
-    using assms(1,2) \<alpha> expand_wp\<^sub>\<alpha> unfolding atomic_rule_def by blast
-next
-  show "guar\<^sub>\<alpha> \<alpha>' (expand\<^sub>G m r G)"
-    using assms(1,2) \<alpha> expand_guar unfolding atomic_rule_def by blast
-qed
-
-section \<open>Auxiliary State\<close>
 
 definition aux\<^sub>P
   where "aux\<^sub>P r P \<equiv> {m. \<exists>m'. (m,m') \<in> r\<^sup>= \<and> m' \<in> P}"
@@ -217,12 +159,9 @@ proof (clarsimp, goal_cases)
   then show ?case using a(1) by auto
 qed
 
-abbreviation aux\<^sub>\<alpha>
-  where "aux\<^sub>\<alpha> r \<alpha> \<equiv> (tag \<alpha>, aux\<^sub>P r (vc \<alpha>), aux\<^sub>R r (beh \<alpha>))"
-
 lemma aux_wp [intro]:
-  assumes "P \<subseteq> wp\<^sub>\<alpha> \<alpha> Q"
-  shows "aux\<^sub>P r P \<subseteq> wp\<^sub>\<alpha> (aux\<^sub>\<alpha> r \<alpha>) (aux\<^sub>P r Q)"
+  assumes "P \<subseteq> wp v b Q"
+  shows "aux\<^sub>P r P \<subseteq> wp (aux\<^sub>P r v) (aux\<^sub>R r b) (aux\<^sub>P r Q)"
   unfolding wp_def aux\<^sub>P_def
 proof (clarsimp, (intro conjI; clarsimp), goal_cases)
   case (1 n m')
@@ -233,229 +172,14 @@ next
 qed
 
 lemma aux_guar [intro]:
-  assumes "guar\<^sub>\<alpha> \<alpha> G" 
-  shows "guar\<^sub>\<alpha> (aux\<^sub>\<alpha> r \<alpha>) (aux\<^sub>G r G)"
+  assumes "guar v b G" 
+  shows "guar (aux\<^sub>P r v) (aux\<^sub>R r b) (aux\<^sub>G r G)"
   unfolding wp_def aux\<^sub>G_def aux\<^sub>P_def aux\<^sub>R_def guar_def
 proof (clarsimp, goal_cases)
   case (1 m m' n)
-  then obtain n' where a: "(m', n') \<in> r\<^sup>=" "(n, n') \<in> beh \<alpha>" by auto
+  then obtain n' where a: "(m', n') \<in> r\<^sup>=" "(n, n') \<in> b" by auto
   hence "(n,n') \<in> G" using assms 1 by (auto simp: guar_def)
-  thus ?case using a(1) 1(3) sorry
+  thus ?case using a(1) 1(2) by auto
 qed
-
-lemma atomic_auxI [intro]:
-  assumes "R,G \<turnstile>\<^sub>A P {\<alpha>} Q" 
-  shows "aux\<^sub>R r R,aux\<^sub>G r G \<turnstile>\<^sub>A aux\<^sub>P r P {aux\<^sub>\<alpha> r \<alpha>} aux\<^sub>P r Q"
-  unfolding atomic_rule_def
-proof (intro conjI)
-  show "stable (aux\<^sub>R r R) (aux\<^sub>P r P)" using assms(1) by (auto simp: atomic_rule_def)
-next
-  show "stable (aux\<^sub>R r R) (aux\<^sub>P r Q)" using assms(1) by (auto simp: atomic_rule_def)
-next
-  have "guar\<^sub>\<alpha> \<alpha> G" using assms(1) by (auto simp: atomic_rule_def)
-  thus "guar\<^sub>\<alpha> (aux\<^sub>\<alpha> r \<alpha>) (aux\<^sub>G r G)" using aux_guar by blast
-next
-  have "P \<subseteq> wp\<^sub>\<alpha> \<alpha> Q" using assms(1) by (auto simp: atomic_rule_def)
-  thus "aux\<^sub>P r P \<subseteq> wp\<^sub>\<alpha> (aux\<^sub>\<alpha> r \<alpha>) (aux\<^sub>P r Q)" using aux_wp by blast
-qed
-
-
-(*
-fun aux\<^sub>c
-  where
-    "aux\<^sub>c r Nil = Nil" |
-    "aux\<^sub>c r (Basic \<alpha>) = (Basic (aux\<^sub>\<alpha> r \<alpha>))" |
-    "aux\<^sub>c r (c\<^sub>1 ; c\<^sub>2) = (aux\<^sub>c r c\<^sub>1 ; aux\<^sub>c r c\<^sub>2)" |
-    "aux\<^sub>c r (c\<^sub>1 \<cdot> c\<^sub>2) = (aux\<^sub>c r c\<^sub>1 \<cdot> aux\<^sub>c r c\<^sub>2)" |
-    "aux\<^sub>c r (c\<^sub>1 \<sqinter> c\<^sub>2)  = (aux\<^sub>c r c\<^sub>1 \<sqinter> aux\<^sub>c r c\<^sub>2)" |
-    "aux\<^sub>c r (Loop c) = Loop (aux\<^sub>c r c)" |
-    "aux\<^sub>c r (BigChoice S\<^sub>1) = (BigChoice ((map (aux\<^sub>\<alpha> r)) ` S\<^sub>1))" |
-    "aux\<^sub>c r (Dec b m c) = (Dec b m (aux\<^sub>c r c))" |
-    "aux\<^sub>c r (c\<^sub>1 || c\<^sub>2) = (aux\<^sub>c r c\<^sub>1 || aux\<^sub>c r c\<^sub>2)"
-
-lemma aux\<^sub>c_nilE [elim!]:
-  assumes "aux\<^sub>c r c = Nil"
-  obtains "c = Nil"
-  using assms
-  by (cases "(r,c)" rule: aux\<^sub>c.cases) auto
-
-lemma aux\<^sub>c_basicE [elim!]:
-  assumes "aux\<^sub>c r c = Basic \<alpha>"
-  obtains \<beta> where "c = Basic \<beta>" "\<alpha> = aux\<^sub>\<alpha> r \<beta>"
-  using assms by (cases "(r,c)" rule: aux\<^sub>c.cases) auto
-
-lemma aux\<^sub>c_seqE [elim!]:
-  assumes "aux\<^sub>c r c = c\<^sub>1 ; c\<^sub>2"
-  obtains c\<^sub>1' c\<^sub>2' where "c = c\<^sub>1' ; c\<^sub>2'" "aux\<^sub>c r c\<^sub>1' = c\<^sub>1" "aux\<^sub>c r c\<^sub>2' = c\<^sub>2"
-  using assms by (cases "(r,c)" rule: aux\<^sub>c.cases) auto
-
-lemma aux\<^sub>c_ordE [elim!]:
-  assumes "aux\<^sub>c r c = c\<^sub>1 \<cdot> c\<^sub>2"
-  obtains c\<^sub>1' c\<^sub>2' where "c = c\<^sub>1' \<cdot> c\<^sub>2'" "aux\<^sub>c r c\<^sub>1' = c\<^sub>1" "aux\<^sub>c r c\<^sub>2' = c\<^sub>2"
-  using assms by (cases "(r,c)" rule: aux\<^sub>c.cases) auto
-
-lemma aux\<^sub>c_choiceE [elim!]:
-  assumes "aux\<^sub>c r c = c\<^sub>1 \<sqinter> c\<^sub>2"
-  obtains c\<^sub>1' c\<^sub>2' where "c = c\<^sub>1' \<sqinter> c\<^sub>2'" "aux\<^sub>c r c\<^sub>1' = c\<^sub>1" "aux\<^sub>c r c\<^sub>2' = c\<^sub>2"
-  using assms by (cases "(r,c)" rule: aux\<^sub>c.cases) auto
-
-lemma aux\<^sub>c_loopE [elim!]:
-  assumes "aux\<^sub>c r c = Loop c\<^sub>1"
-  obtains c\<^sub>1' where "c = Loop c\<^sub>1'" "aux\<^sub>c r c\<^sub>1' = c\<^sub>1" 
-  using assms by (cases "(r,c)" rule: aux\<^sub>c.cases) auto
-
-lemma aux_local [intro]:
-  assumes "local c" 
-  shows "local (aux\<^sub>c r c)"
-  using assms by (induct c rule: local.induct) auto
-*)
-
-(*
-lemma aux\<^sub>c_seqE2 [elim!]:
-  assumes "c\<^sub>1 ; c\<^sub>2 = aux\<^sub>c r c "
-  obtains c\<^sub>1' c\<^sub>2' where "c = c\<^sub>1' ; c\<^sub>2'" "aux\<^sub>c r c\<^sub>1' = c\<^sub>1" "aux\<^sub>c r c\<^sub>2' = c\<^sub>2"
-  using assms by (cases "(r,c)" rule: aux\<^sub>c.cases) auto
-
-lemma aux\<^sub>c_ordE [elim!]:
-  assumes "c\<^sub>1 \<cdot> c\<^sub>2 = aux\<^sub>c r c"
-  obtains c\<^sub>1' c\<^sub>2' where "c = c\<^sub>1' \<cdot> c\<^sub>2'" "aux\<^sub>c r c\<^sub>1' = c\<^sub>1" "aux\<^sub>c r c\<^sub>2' = c\<^sub>2"
-  using assms by (cases "(r,c)" rule: aux\<^sub>c.cases) auto
-
-lemma aux\<^sub>c_parE [elim!]:
-  assumes "c\<^sub>1 || c\<^sub>2 = aux\<^sub>c r c"
-  obtains c\<^sub>1' c\<^sub>2' where "c = c\<^sub>1' || c\<^sub>2'" "aux\<^sub>c r c\<^sub>1' = c\<^sub>1" "aux\<^sub>c r c\<^sub>2' = c\<^sub>2"
-  using assms by (cases "(r,c)" rule: aux\<^sub>c.cases) auto
-
-lemma aux\<^sub>c_choiceE [elim!]:
-  assumes "c\<^sub>1 \<sqinter> c\<^sub>2 = aux\<^sub>c r c"
-  obtains c\<^sub>1' c\<^sub>2' where "c = c\<^sub>1' \<sqinter> c\<^sub>2'" "aux\<^sub>c r c\<^sub>1' = c\<^sub>1" "aux\<^sub>c r c\<^sub>2' = c\<^sub>2"
-  using assms by (cases "(r,c)" rule: aux\<^sub>c.cases) auto
-
-lemma aux\<^sub>c_loopE [elim!]:
-  assumes "Loop c\<^sub>1 = aux\<^sub>c r c"
-  obtains c\<^sub>1' where "c = Loop c\<^sub>1'" "aux\<^sub>c r c\<^sub>1' = c\<^sub>1" 
-  using assms by (cases "(r,c)" rule: aux\<^sub>c.cases) auto
-
-lemma aux\<^sub>c_bigchoiceE [elim!]:
-  assumes "(\<Sqinter> S) = aux\<^sub>c r c"
-  obtains S' where "c = \<Sqinter> S'" "S = (map (aux\<^sub>\<alpha> r)) ` S'" 
-  using assms by (cases "(r,c)" rule: aux\<^sub>c.cases) auto
-
-lemma [simp]:
-  "seq2com (map (aux\<^sub>\<alpha> r) x) = aux\<^sub>c r (seq2com x)"
-proof (induct x)
-case Nil
-  then show ?case by auto
-next
-  case (Cons a x)
-  then show ?case  by auto
-qed
-
-lemma aux_rewriteE:
-  assumes "aux\<^sub>c r c \<leadsto> c\<^sub>a"
-  obtains c' where "c \<leadsto> c'" "aux\<^sub>c r c' = c\<^sub>a"
-  using assms
-  by (induct "aux\<^sub>c r c" c\<^sub>a arbitrary: r c) (auto; force)+
-
-lemma aux\<^sub>c_basicE [elim!]:
-  assumes "Basic \<alpha> = aux\<^sub>c r c"
-  obtains \<beta> where "c = Basic \<beta>" "\<alpha> = aux\<^sub>\<alpha> r \<beta>"
-  using assms by (cases "(r,c)" rule: aux\<^sub>c.cases) auto
-
-lemma [simp]:
-  "(aux\<^sub>\<alpha> r \<beta>)\<langle>tag x\<rangle> = aux\<^sub>\<alpha> r \<beta>\<langle>tag x\<rangle>"
-  
-  sorry
-
-lemma [simp]:
-  "(aux\<^sub>\<alpha> r \<beta>)\<llangle>aux\<^sub>c r p\<rrangle> = aux\<^sub>\<alpha> r \<beta>\<llangle>p\<rrangle>"
-  by (induct p arbitrary: \<beta>) auto
-
-lemma aux_re:
-  assumes "\<alpha>' < aux\<^sub>c r c <\<^sub>c aux\<^sub>\<alpha> r \<alpha>"
-  obtains \<beta> where "\<beta> < c <\<^sub>c \<alpha>" "\<alpha>' = aux\<^sub>\<alpha> r \<beta>"
-  using assms
-proof (induct c arbitrary: \<alpha>' \<alpha>)
-  case Nil
-  then show ?case by auto
-next
-  case (Basic x)
-  hence "tag x \<hookleftarrow> tag (\<alpha>)\<langle>tag x\<rangle>" by auto
-  moreover have "\<alpha>' = aux\<^sub>\<alpha> r \<alpha>\<langle>tag x\<rangle>" using Basic(2) by auto
-  ultimately show ?case using Basic(1) by auto
-next
-  case (Seq c1 c2)
-  then obtain \<beta> where b: "\<alpha>' < aux\<^sub>c r c1 <\<^sub>c \<beta>" "\<beta> < aux\<^sub>c r c2 <\<^sub>c aux\<^sub>\<alpha> r \<alpha>" by auto
-  show ?case 
-  proof (rule Seq(2)[OF _ b(2)])
-    fix \<beta>' assume c: "\<beta>' < c2 <\<^sub>c \<alpha>" "\<beta> = aux\<^sub>\<alpha> r \<beta>'"
-    hence a: "\<alpha>' < aux\<^sub>c r c1 <\<^sub>c aux\<^sub>\<alpha> r \<beta>'" using b by auto
-    show ?thesis apply (rule Seq(1)[OF _a]) using c(1) Seq(3) reorder_com.simps(3) by blast 
-  qed
-next
-  case (Ord c1 c2)
-  then obtain \<beta> where b: "\<alpha>' < aux\<^sub>c r c1 <\<^sub>c \<beta>" "\<beta> < aux\<^sub>c r c2 <\<^sub>c aux\<^sub>\<alpha> r \<alpha>" by auto
-  show ?case 
-  proof (rule Ord(2)[OF _ b(2)])
-    fix \<beta>' assume c: "\<beta>' < c2 <\<^sub>c \<alpha>" "\<beta> = aux\<^sub>\<alpha> r \<beta>'"
-    hence a: "\<alpha>' < aux\<^sub>c r c1 <\<^sub>c aux\<^sub>\<alpha> r \<beta>'" using b by auto
-    show ?thesis apply (rule Ord(1)[OF _a]) using c(1) Ord(3) reorder_com.simps(4) by blast 
-  qed
-qed auto
-
-lemma aux_execE:
-  assumes "aux\<^sub>c r c \<mapsto>[p,\<alpha>] c\<^sub>a"
-  obtains c' p' \<beta> where "c \<mapsto>[p',\<beta>] c'" "aux\<^sub>c r c' = c\<^sub>a" "\<alpha> = aux\<^sub>\<alpha> r \<beta>" "aux\<^sub>c r p' = p"
-  using assms
-proof (induct "aux\<^sub>c r c" p \<alpha> c\<^sub>a arbitrary: r c)
-  case (act \<alpha>)
-  then show ?case apply auto by force
-next
-  case (seq c\<^sub>1 r' \<alpha> c\<^sub>1' c\<^sub>2)
-  then show ?case apply auto by force
-next
-  case (ord c\<^sub>1 r \<alpha> c\<^sub>1' c\<^sub>2)
-  then show ?case apply auto by force
-next
-  case (ooo c\<^sub>2 r' \<alpha> c\<^sub>2' \<alpha>' c\<^sub>1)
-  then obtain c\<^sub>1' c' where s: "c = c\<^sub>1' ; c'" "c\<^sub>1 = aux\<^sub>c r c\<^sub>1'" "aux\<^sub>c r c' = c\<^sub>2" by auto
-
-  
-  show ?case 
-  proof (rule ooo(2)[of r c'], goal_cases)
-    case 1
-    then show ?case using s by auto
-  next
-    case (2 p' \<beta> c'')
-    hence re: "\<alpha>' < aux\<^sub>c r (c\<^sub>1' ; p') <\<^sub>c aux\<^sub>\<alpha> r \<beta>" using ooo(3) s by auto
-    then obtain \<beta>' where b: "\<beta>' < c\<^sub>1' ; p' <\<^sub>c \<beta>" using aux_re by blast
-
-    show ?case 
-      apply (rule ooo(5)[of "c\<^sub>1' ; p'" \<beta> "c\<^sub>1' ; c''"])
-      using s 2 b apply auto
-      apply (rule execute.ooo[of _ _ _ _ \<beta>'], simp)
-      by auto
-  qed 
-next
-  case (par1 c\<^sub>1 r' \<alpha> c\<^sub>1' c\<^sub>2)
-  then show ?case apply auto by force
-next
-  case (par2 c\<^sub>2 r' \<alpha> c\<^sub>2' c\<^sub>1)
-  then show ?case apply auto by force
-qed *)
-
-*)
-
-(* next
-  case (aux R G P c Q r')
-  thus ?case sorry then obtain c'' p' \<beta> where a: "c \<mapsto>[p',\<beta>] c''" "aux\<^sub>c r' c'' = c'" "\<alpha> = aux\<^sub>\<alpha> r' \<beta>" "r = aux\<^sub>c r' p'"
-    apply (elim aux_execE) by blast
-  then obtain P' M where p: "P \<subseteq> P'" "R,G \<turnstile>\<^sub>A P' {\<beta>\<llangle>p'\<rrangle>} M" "R,G \<turnstile> M {c''} Q"
-    using aux(2)[OF a(1)] by blast
-  have "aux\<^sub>P r' P \<subseteq> aux\<^sub>P r' P'" using p by (simp add: aux\<^sub>P_mono)
-  moreover have "aux\<^sub>R r' R,aux\<^sub>G r' G \<turnstile> aux\<^sub>P r' M {c'} aux\<^sub>P r' Q" using p  a(2) by blast
-  moreover have "aux\<^sub>R r' R,aux\<^sub>G r' G \<turnstile>\<^sub>A aux\<^sub>P r' P' {\<alpha>\<llangle>r\<rrangle>} aux\<^sub>P r' M"
-    using p(2) unfolding a by simp blast
-  ultimately show ?case by blast*)
 
 end
