Transition_Rules.thy
@@ -120,6 +120,27 @@ proof (induct arbitrary: c' rule: rules.induct)
 next
   case (ord R G P c\<^sub>1 Q c\<^sub>2 M)
   thus ?case by (cases rule: silentE, auto) blast+
+next
+  case (refine R G P c\<^sub>1 Q c\<^sub>2)
+  thus ?case using syntax_rel_silent by force
+next
+  case (aux R G P c Q r c'')
+  thus ?case using syntax_rel_silent rules.aux by metis
+next
+  case (thread R G P c Q l op)
+  thus ?case 
+  proof (cases rule: silentE, auto, goal_cases)
+    case (1 M)
+    have "thr\<^sub>R l R,thr\<^sub>G l G \<turnstile> thr\<^sub>P l op M {Nil} thr\<^sub>P l op M"
+      apply (rule rules.nil)
+      using thr_stable 1 by metis
+    then show ?case
+      apply (rule conseq)
+      using 1 thr_mono apply metis
+      apply simp
+      apply simp
+      using 1 unfolding thr\<^sub>P_def thr\<^sub>Q_def by auto
+  qed
 qed (cases rule: silentE, auto)+
 
 text \<open>Judgements are preserved across thread-local execution steps\<close>
@@ -188,7 +209,7 @@ next
   then obtain M v where p: "P \<subseteq> wp v g M" "guar v g G" "R,G \<turnstile> M {c'} Q" by metis
   hence "P \<inter> M' \<subseteq> wp v g (M \<inter> M')" using inv(3,4) by (auto simp: stable_def guar_def wp_def) blast
   thus ?case using rules.inv p(2,3) inv(3,4) by blast
-next       
+next
   case (thread R G P c Q op l)
   \<comment> \<open>Convert the global execution step into a local execution step\<close>
   obtain r \<alpha> c\<^sub>t l' where thr: "g = thr2glb op l l' (beh \<alpha>\<llangle>r\<rrangle>)" "c' = Thread l' op c\<^sub>t" "c \<mapsto>[r,\<alpha>] c\<^sub>t"
@@ -205,6 +226,23 @@ next
   moreover have "guar (thr\<^sub>P op l (vc \<alpha>\<llangle>r\<rrangle>)) g (thr\<^sub>G op G)"
     using p(2) thr_guar thr(1) by fast
   ultimately show ?case using p i unfolding thr(2) by blast
+next
+  case (refine R G P c\<^sub>1 Q c\<^sub>2)
+  then obtain c\<^sub>1' g' where g: "g' \<supseteq> g" "c\<^sub>1 \<mapsto>[g'] c\<^sub>1'" "refine c\<^sub>1' c'"
+    using refine_global[OF refine(3,4)] by auto
+  thus ?case using refine(2)[OF g(2)] rules.refine wp_conseqI guar_conseqI 
+    by (metis order_refl) 
+next
+  case (aux R G P c\<^sub>1 Q r c\<^sub>2)
+  then obtain c\<^sub>1' g' where g: "g \<subseteq> aux\<^sub>R r g'" "c\<^sub>1 \<mapsto>[g'] c\<^sub>1'" "aux\<^sub>C r c\<^sub>1' c'"
+    using aux_global[OF aux(3,4)] by auto
+  then obtain M v where m: "P \<subseteq> wp v g' M" "guar v g' G" "R,G \<turnstile> M {c\<^sub>1'} Q"
+    using aux(2) by metis
+  show ?case 
+    using rules.aux[OF m(3) g(3)] 
+    using wp_conseqI[OF aux_wp[OF m(1), of r] g(1)]
+    using guar_conseqI[OF aux_guar[OF m(2), of r] g(1)]
+    by auto
 qed auto
 
 end
